

# Kinematics Final Assignment

Haniyeh Zahra Budaqi  
haniyehz.budaqi55@sharif.edu

December 12, 2025

## Problem Two

Using the  $[B(\sigma)]$  matrix of the MRP differential kinematic equations,

$$[B(\sigma)] = (1 - \sigma^2)[I_{3 \times 3}] + 2[\tilde{\sigma}] + 2\sigma\sigma^T$$

develop the simple inverse expression for  $[B]^{-1}$ .

Note the identity  $[\tilde{\sigma}]^2 = \sigma\sigma^T - \sigma^2[I_{3 \times 3}]$

Hint: investigate what happens to  $[B][B]^T$

## Answer

Let us first make the matrix  $[B]^T$ :

$$\begin{aligned}[B]^T &= [(1 - \sigma^2)[I_{3 \times 3}] + 2[\tilde{\sigma}] + 2\sigma\sigma^T]^T \\ &= [(1 - \sigma^2)[I_{3 \times 3}]]^T + 2[\tilde{\sigma}]^T + 2[\sigma\sigma^T]^T\end{aligned}$$

From the three terms above, only  $[\tilde{\sigma}]$  is skew-symmetric, for which we have:

$$[\tilde{\sigma}]^T = -[\tilde{\sigma}]$$

and so we have:

$$[B]^T = (1 - \sigma^2)[I_{3 \times 3}] - 2[\tilde{\sigma}] + 2\sigma\sigma^T$$

Now we investigate what happens to  $[B][B]^T$ :

$$\begin{aligned}[B][B]^T &= [(1 - \sigma^2)[I_{3 \times 3}] + 2[\tilde{\sigma}] + 2\sigma\sigma^T][(1 - \sigma^2)[I_{3 \times 3}] - 2[\tilde{\sigma}] + 2\sigma\sigma^T] \\ &= (1 - \sigma^2)^2[I_{3 \times 3}] - 2(1 - \sigma^2)[\tilde{\sigma}] + 2(1 - \sigma^2)\sigma\sigma^T \\ &\quad + 2(1 - \sigma^2)[\tilde{\sigma}] - 4[\tilde{\sigma}]^2 + 4[\tilde{\sigma}]\sigma\sigma^T \\ &\quad + 2(1 - \sigma^2)\sigma\sigma^T + 4\sigma\sigma^T[\tilde{\sigma}] + 4(\sigma\sigma^T)^2\end{aligned}$$

Looking at the derived expressions, we see that  $-2(1 - \sigma^2)[\tilde{\sigma}] + 2(1 - \sigma^2)[\tilde{\sigma}] = 0$  and also  $4[\tilde{\sigma}]\sigma\sigma^T = 4\sigma\sigma^T[\tilde{\sigma}] = 0$ . Worth noting that  $4(\sigma\sigma^T)^2 = 4[\sigma(\sigma^T\sigma)\sigma^T]$  and turns to  $4\sigma^2[\sigma\sigma^T]$ . Rewriting the remaining expressions we have:

$$\begin{aligned}[B][B]^T &= [(1 - \sigma^2)^2[I_{3 \times 3}] + 4(1 - \sigma^2)[\sigma\sigma^T] - 4[\tilde{\sigma}] + 4\sigma^2[\sigma\sigma^T]] \\ &= [(1 - \sigma^2)^2[I_{3 \times 3}] + 4[\sigma\sigma^T] - 4\sigma^2[\sigma\sigma^T] - 4[\tilde{\sigma}] + 4\sigma^2[\sigma\sigma^T]] \\ &= [(1 - \sigma^2)^2[I_{3 \times 3}] + 4[\sigma\sigma^T] - 4[\tilde{\sigma}]]\end{aligned}$$

From the identity  $[\tilde{\sigma}]^2 = \sigma\sigma^T - \sigma^2[I_{3 \times 3}]$ , we put in  $[\tilde{\sigma}]$ :

$$\begin{aligned}
 [B][B]^T &= [(1 - \sigma^2)^2[I_{3 \times 3}] + 4[\sigma\sigma^T] - 4[\sigma\sigma^T - \sigma^2[I_{3 \times 3}]] \\
 &= (1 - \sigma^2)^2[I_{3 \times 3}] + 4[\sigma\sigma^T] - 4[\sigma\sigma^T] + 4\sigma^2[I_{3 \times 3}] \\
 &= ((1 - \sigma^2)^2 + 4\sigma^2)[I_{3 \times 3}] \\
 &= (1 - 2\sigma^2 + \sigma^4 + 4\sigma^2)[I_{3 \times 3}] = (1 + 2\sigma^2 + \sigma^4)[I_{3 \times 3}] \\
 &= (1 + \sigma^2)^2[I_{3 \times 3}]
 \end{aligned}$$

We end up with:

$$[B][B]^T = (1 + \sigma^2)^2[I_{3 \times 3}]$$

So:

$$\begin{aligned}
 [B]\left(\frac{1}{(1 + \sigma^2)^2}[B]^T\right) &= [I_{3 \times 3}] \\
 \Rightarrow [B]^{-1} &= \frac{1}{(1 + \sigma^2)^2}[B]^T
 \end{aligned}$$